src/parser/FStarC.Parser.Const.ExtractAs.fst
@@ -1,0 +1,38 @@
+(*
+   Copyright 2008-2025 Nikhil Swamy and Microsoft Research
+
+   Licensed under the Apache License, Version 2.0 (the "License");
+   you may not use this file except in compliance with the License.
+   You may obtain a copy of the License at
+
+       http://www.apache.org/licenses/LICENSE-2.0
+
+   Unless required by applicable law or agreed to in writing, software
+   distributed under the License is distributed on an "AS IS" BASIS,
+   WITHOUT WARRANTIES OR C  ONDITIONS OF ANY KIND, either express or implied.
+   See the License for the specific language governing permissions and
+   limitations under the License.
+*)
+module FStarC.Parser.Const.ExtractAs
+
+open FStarC
+open FStarC.Effect
+open FStarC.Util
+open FStarC.Ident
+open FStarC.Range.Type
+open FStarC.Const
+open FStarC.Syntax
+open FStarC.Syntax.Syntax
+
+let p2l l = lid_of_path l dummyRange
+let extract_as_lid = p2l ["FStar"; "ExtractAs"; "extract_as"]
+
+let is_extract_as_attr (attr: attribute) : option term =
+  let head, args = Syntax.Util.head_and_args attr in
+  match (Subst.compress head).n, args with
+  | Tm_fvar fv, [t, _] when Syntax.fv_eq_lid fv extract_as_lid ->
+    (match (Subst.compress t).n with
+    | Tm_quoted(impl, _) -> Some impl
+    | _ -> None)
+  | _ -> None
+
