src/parser/FStarC.Parser.Const.ExtractAs.fsti
@@ -1,0 +1,25 @@
+(*
+   Copyright 2008-2025 Nikhil Swamy and Microsoft Research
+
+   Licensed under the Apache License, Version 2.0 (the "License");
+   you may not use this file except in compliance with the License.
+   You may obtain a copy of the License at
+
+       http://www.apache.org/licenses/LICENSE-2.0
+
+   Unless required by applicable law or agreed to in writing, software
+   distributed under the License is distributed on an "AS IS" BASIS,
+   WITHOUT WARRANTIES OR C  ONDITIONS OF ANY KIND, either express or implied.
+   See the License for the specific language governing permissions and
+   limitations under the License.
+*)
+module FStarC.Parser.Const.ExtractAs
+
+open FStarC
+open FStarC.Effect
+open FStarC.Ident
+open FStarC.Syntax.Syntax
+
+val extract_as_lid : lid
+
+val is_extract_as_attr (attr: attribute) : option term
